\section{Small-Step \ce} \label{sec:mach}
Using the big-step \ce from the previous section, we construct a small-step
semantics by adding a stack.  The syntax and semantics are defined in
Figure~\ref{fig:cesm}. 

\begin{figure}
\textbf{Syntax}
\begin{align*}
\tag{State} s &::= \langle c, \sigma, \mu \rangle \\
\tag{Term} t &::= i \; | \; \lambda t \; | \; t \; t  \\
\tag{Variable} i &\in \mathbb{N}  \\
\tag{Closure} c &::= t \left[l\right] \\
\tag{Value} v &::= \lambda t\left[l\right] \\
\tag{Heap} \mu &::= \epsilon \; | \; \mu \left[ l \mapsto \rho \right] \\
\tag{Environment} \rho &::= \bullet \; | \; c \cdot l \\
\tag{Stack} \sigma &::= \square \; | \; \sigma \; c \;  | \; \sigma \; u \\
\tag{Location} l,u,f &\in \mathbb{N}
\end{align*}
\textbf{Semantics}
\begin{align*}
\tag{Upd}
\langle v,  \sigma \; u , \mu \rangle 
  &\rightarrow
\langle v, \sigma, \mu\left(u \mapsto v \cdot l\right) \rangle  
\; \textnormal{where} \; c \cdot l = \mu\left(u\right) \\
\tag{Lam}
\langle \lambda t\left[l\right], \sigma \; c, \mu \rangle 
  &\rightarrow
\langle t\left[f\right], \sigma, \mu\left[f \mapsto c \cdot l\right]\rangle f
\not \in \textnormal{dom}\left(\mu\right)  \\
\tag{App}
\langle t \; t'\left[l\right], \sigma, \mu \rangle
  &\rightarrow
\langle t\left[l\right], \sigma \; t'\left[l\right], \mu \rangle \\
\tag{Var}
\langle i\left[l\right], \sigma, \mu \rangle
  &\rightarrow
\langle c, \sigma \; l'', \mu \rangle
\; \textnormal{where} \; l'' \mapsto c \cdot l' = \mu\left(l, i\right)
\end{align*}
\caption{Small-step \ce syntax and semantics}
\label{fig:cesm}
\end{figure}

The small-step semantics operate identically to the big-step, extended only with
a context (or stack) to implement the updates from the Id subderivation ($\sigma
\; u$) and the operands from the App subderivation ($\sigma \; c$).  Much like
the big-step semantics, a term $t$ is inserted into an initial state $\langle
t[0], \sigma, \epsilon[0\mapsto\bullet]\rangle$ . For the update rule, the
current closure is a value, and there is an update marker as the outermost
context.  This implies that a variable was entered and that the current closure
represents the corresponding value for that variable. Thus, we update the
location $u$ that the variable entered, replacing whatever closure was entered
with the current closure.  The Lam rule takes an argument off the context and
binds it to a variable, allocating a fresh heap location for the bound variable.
This ensures that every instance of the variable will point to this location,
and thus the bound closure will be evaluated at most once. The App rule simply
pushes the argument term in the current environment. The Var rule enters the
closure pointed to by the \textit{i}'th environment location.  

\sloppy To get some intuition for the \ce machine and how it works, please refer
to Figure~\ref{fig:state}, which displays the steps in the evaluation of the
term \\ $(\lambda a.(\lambda b.b \; a) \lambda c.c \; a) \; ((\lambda i.i)
\lambda j.j)$, or $(\lambda(\lambda0\;1)\;\lambda0\;1)\;((\lambda0)\; \lambda0)$
with de Bruijn indices.

\begin{sidewaysfigure}
\begin{align*}
&\langle (\lambda(\lambda0\;1)\;\lambda0\;1)\;((\lambda0)\;\lambda0)[0],\square,\epsilon[0\mapsto\bullet]\rangle\\
&\rightarrow\langle \lambda(\lambda0\;1)\;\lambda0\;1[0],\square (\lambda0)\;\lambda0[0],\epsilon[0\mapsto\bullet]\rangle\\ 
&\rightarrow\langle (\lambda0\;1)\;\lambda0\;1[1],\square,\epsilon[0\mapsto\bullet][1\mapsto(\lambda0)\;\lambda0[0]\cdot0]\rangle\\ 
&\rightarrow\langle \lambda0\;1[1],\square \lambda0\;1[1],\epsilon[0\mapsto\bullet][1\mapsto(\lambda0)\;\lambda0[0]\cdot0]\rangle\\ 
&\rightarrow\langle 0\;1[2],\square,\epsilon[0\mapsto\bullet][1\mapsto(\lambda0)\;\lambda0[0]\cdot0][2\mapsto\lambda0\;1[1]\cdot1]\rangle\\ 
&\rightarrow\langle 0[2],\square 1[2],\epsilon[0\mapsto\bullet][1\mapsto(\lambda0)\;\lambda0[0]\cdot0][2\mapsto\lambda0\;1[1]\cdot1]\rangle\\ 
&\rightarrow\langle \lambda0\;1[1],\square 1[2] 2,\epsilon[0\mapsto\bullet][1\mapsto(\lambda0)\;\lambda0[0]\cdot0][2\mapsto\lambda0\;1[1]\cdot1]\rangle\\ 
&\rightarrow\langle \lambda0\;1[1],\square 1[2],\epsilon[0\mapsto\bullet][1\mapsto(\lambda0)\;\lambda0[0]\cdot0][2\mapsto\lambda0\;1[1]\cdot1]\rangle\\ 
&\rightarrow\langle 0\;1[3],\square,\epsilon[0\mapsto\bullet][1\mapsto(\lambda0)\;\lambda0[0]\cdot0][2\mapsto\lambda0\;1[1]\cdot1][3\mapsto1[2]\cdot1]\rangle\\ 
&\rightarrow\langle 0[3],\square 1[3],\epsilon[0\mapsto\bullet][1\mapsto(\lambda0)\;\lambda0[0]\cdot0][2\mapsto\lambda0\;1[1]\cdot1][3\mapsto1[2]\cdot1]\rangle\\ 
&\rightarrow\langle 1[2],\square 1[3] 3,\epsilon[0\mapsto\bullet][1\mapsto(\lambda0)\;\lambda0[0]\cdot0][2\mapsto\lambda0\;1[1]\cdot1][3\mapsto1[2]\cdot1]\rangle\\ 
&\rightarrow\langle 0[1],\square 1[3] 3,\epsilon[0\mapsto\bullet][1\mapsto(\lambda0)\;\lambda0[0]\cdot0][2\mapsto\lambda0\;1[1]\cdot1][3\mapsto1[2]\cdot1]\rangle\\ 
\end{align*}
\caption{Small-step \ce example. Evaluation of
$(\lambda(\lambda0\;1)\;\lambda0\;1)\;((\lambda0)\;\lambda0)$}
\end{sidewaysfigure}

\begin{sidewaysfigure}
\ContinuedFloat
\begin{align*}
&\rightarrow \langle (\lambda0)\;\lambda0[0],\square 1[3] 3 1,\epsilon[0\mapsto\bullet][1\mapsto(\lambda0)\;\lambda0[0]\cdot0][2\mapsto\lambda0\;1[1]\cdot1][3\mapsto1[2]\cdot1]\rangle\\ 
&\rightarrow \langle \lambda0[0],\square 1[3] 3 1 \lambda0[0],\epsilon[0\mapsto\bullet][1\mapsto(\lambda0)\;\lambda0[0]\cdot0][2\mapsto\lambda0\;1[1]\cdot1][3\mapsto1[2]\cdot1]\rangle\\ 
&\rightarrow\langle 0[4],\square 1[3] 3 1,\epsilon[0\mapsto\bullet][1\mapsto(\lambda0)\;\lambda0[0]\cdot0][2\mapsto\lambda0\;1[1]\cdot1][3\mapsto1[2]\cdot1][4\mapsto\lambda0[0]\cdot0]\rangle\\ 
&\rightarrow\langle \lambda0[0],\square 1[3] 3 1 4,\epsilon[0\mapsto\bullet][1\mapsto(\lambda0)\;\lambda0[0]\cdot0][2\mapsto\lambda0\;1[1]\cdot1][3\mapsto1[2]\cdot1][4\mapsto\lambda0[0]\cdot0]\rangle\\ 
&\rightarrow\langle \lambda0[0],\square 1[3] 3 1,\epsilon[0\mapsto\bullet][1\mapsto(\lambda0)\;\lambda0[0]\cdot0][2\mapsto\lambda0\;1[1]\cdot1][3\mapsto1[2]\cdot1][4\mapsto\lambda0[0]\cdot0]\rangle\\ 
&\rightarrow\langle \lambda0[0],\square 1[3] 3,\epsilon[0\mapsto\bullet][1\mapsto\lambda0[0]\cdot0][2\mapsto\lambda0\;1[1]\cdot1][3\mapsto1[2]\cdot1][4\mapsto\lambda0[0]\cdot0]\rangle\\ 
&\rightarrow\langle \lambda0[0],\square 1[3],\epsilon[0\mapsto\bullet][1\mapsto\lambda0[0]\cdot0][2\mapsto\lambda0\;1[1]\cdot1][3\mapsto\lambda0[0]\cdot1][4\mapsto\lambda0[0]\cdot0]\rangle\\ 
&\rightarrow\langle 0[5],\square,\epsilon[0\mapsto\bullet][1\mapsto\lambda0[0]\cdot0][2\mapsto\lambda0\;1[1]\cdot1][3\mapsto\lambda0[0]\cdot1][4\mapsto\lambda0[0]\cdot0][5\mapsto1[3]\cdot0]\rangle\\ 
&\rightarrow\langle 1[3],\square 5,\epsilon[0\mapsto\bullet][1\mapsto\lambda0[0]\cdot0][2\mapsto\lambda0\;1[1]\cdot1][3\mapsto\lambda0[0]\cdot1][4\mapsto\lambda0[0]\cdot0][5\mapsto1[3]\cdot0]\rangle\\ 
&\rightarrow\langle 0[1],\square 5,\epsilon[0\mapsto\bullet][1\mapsto\lambda0[0]\cdot0][2\mapsto\lambda0\;1[1]\cdot1][3\mapsto\lambda0[0]\cdot1][4\mapsto\lambda0[0]\cdot0][5\mapsto1[3]\cdot0]\rangle\\ 
&\rightarrow\langle \lambda0[0],\square 5 1,\epsilon[0\mapsto\bullet][1\mapsto\lambda0[0]\cdot0][2\mapsto\lambda0\;1[1]\cdot1][3\mapsto\lambda0[0]\cdot1][4\mapsto\lambda0[0]\cdot0][5\mapsto1[3]\cdot0]\rangle\\ 
&\rightarrow\langle \lambda0[0],\square 5,\epsilon[0\mapsto\bullet][1\mapsto\lambda0[0]\cdot0][2\mapsto\lambda0\;1[1]\cdot1][3\mapsto\lambda0[0]\cdot1][4\mapsto\lambda0[0]\cdot0][5\mapsto1[3]\cdot0]\rangle\\ 
&\rightarrow\langle \lambda0[0],\square,\epsilon[0\mapsto\bullet][1\mapsto\lambda0[0]\cdot0][2\mapsto\lambda0\;1[1]\cdot1][3\mapsto\lambda0[0]\cdot1][4\mapsto\lambda0[0]\cdot0][5\mapsto\lambda0[0]\cdot0]\rangle
\end{align*}
\caption{Small-step \ce example. Evaluation of
$(\lambda(\lambda0\;1)\;\lambda0\;1)\;((\lambda0)\;\lambda0)$ (cont.)}
\label{fig:state}
\end{sidewaysfigure}

